send_to

interface_abstraction/Network.thy
@@ -71,6 +71,16 @@ section{*A network consisting of entities*}
         done
     end
 
+   subsection{*Selecting hosts and NetworkBoxes*}
+    text{*select all hosts in an interface set*}
+    definition hosts :: "'v interface set \<Rightarrow> 'v interface set" where
+      "hosts ifaces \<equiv> {e \<in> ifaces. \<exists> x. entity e = Host x}"
+    (*hosts only contains hosts*)
+    lemma "entity ` hosts ifaces = Host ` entity_name ` entity ` hosts ifaces"
+      apply(simp add: hosts_def image_def)
+      apply(rule Set.Collect_cong)
+      apply(simp add: entity_name_def)
+      by fastforce
 
     subsection{*Moving packets*}
       text{*The following simple model is used. A packet is moved from input interface to input interface.
@@ -307,10 +317,12 @@ section{*A network consisting of entities*}
      "\<lbrakk> wellformed_network N; start \<in> interfaces N \<rbrakk> \<Longrightarrow> reachable N hdr start = (\<Union> first_hop \<in> succ N start. {dst. (first_hop, dst) \<in> (view N hdr)\<^sup>+}) \<union> (succ N start)"
      by(simp add: reachable_eq_rtrancl_view start_view_rtrancl)
 
+
+
   section{*Sending packets to hosts*}
     text{*a packet from start is sent to dst. Which hosts gets the packet?*}
     definition send_to :: "'v network \<Rightarrow> 'v interface \<Rightarrow> 'v entity \<Rightarrow> 'v interface set" where
-      "send_to N start dst \<equiv> {e \<in> reachable N (entity start, dst) start. \<exists> x. entity e = Host x}"
+      "send_to N start dst \<equiv> hosts (reachable N (entity start, dst) start)"
 
 
 section{*TEST TEST TES TEST of UNIO*}
