interface_abstraction/Network_ex.thy
@@ -220,26 +220,43 @@ section{*Another example*}
   text{*Carl to Alice*}
   value "reachable_code example_network2 (Host ''Carl'', Host ''Alice'') \<lparr>entity = Host ''Carl'', port = Port 1\<rparr>"
 
+  section{*selecotrs*}
+    lemma [code_unfold]: "hosts ifaces = {e \<in> ifaces. (case entity e of Host _ \<Rightarrow> True | _ \<Rightarrow> False)}"
+      apply(simp add: hosts_def)
+      apply(rule Set.Collect_cong)
+      apply(rule)
+      apply(simp)
+      apply(case_tac "entity e")
+      apply(simp)
+      apply(simp)
+      apply(simp)
+      apply(case_tac "entity e")
+      by auto
+  lemma "hosts (interfaces example_network2) = 
+    {\<lparr>entity = Host ''Alice'', port = Port 1\<rparr>, \<lparr>entity = Host ''Bob'', port = Port 1\<rparr>, \<lparr>entity = Host ''Carl'', port = Port 1\<rparr>, \<lparr>entity = Host ''Dan'', port = Port 1\<rparr>}" by eval
+
+
   section{*send_to*}
     definition send_to_code :: "'v network \<Rightarrow> 'v interface \<Rightarrow> 'v entity \<Rightarrow> 'v interface set" where
-      "send_to_code N start dst \<equiv> Set.filter (\<lambda>e. case entity e of Host _ \<Rightarrow> True | _ \<Rightarrow> False) (reachable_code N (entity start, dst) start)"
+      "send_to_code N start dst \<equiv> hosts (reachable_code N (entity start, dst) start)"
   lemma send_to_code_correct: "wellformed_network N \<Longrightarrow> start \<in> interfaces N \<Longrightarrow> 
     send_to_code N start dst = send_to N start dst"
-    apply(simp add: send_to_code_def send_to_def reachable_code_correct Set.filter_def)
-    apply(rule Set.Collect_cong)
-    apply(rule)
-    apply(simp)
-    apply(case_tac "entity a")
-    apply(simp)
-    apply(simp)
-    apply(simp)
-    apply(clarify)
-    by auto
+    by(simp add: send_to_code_def send_to_def reachable_code_correct Set.filter_def)
 
     text{*in network one, carl and bob are at the same port, our packet arrives at both*}
     lemma "send_to_code example_network \<lparr>entity = Host ''Alice'', port = Port 1\<rparr> (Host ''Carl'') = {\<lparr>entity = Host ''Carl'', port = Port 1\<rparr>, \<lparr>entity = Host ''Bob'', port = Port 1\<rparr>}" by eval
     text{*network two makes sure that the packet only arrives at carl*}
     lemma "send_to_code example_network2 \<lparr>entity = Host ''Alice'', port = Port 1\<rparr> (Host ''Carl'') = {\<lparr>entity = Host ''Carl'', port = Port 1\<rparr>}" by eval
+
+    text{*if switch 1 sends out a packet at port 1, it is directly deliverd via the physical link to Alice. There, the packet ends. *}
+    lemma "send_to_code example_network2 \<lparr> entity = NetworkBox ''sw1'', port = Port 1 \<rparr> (Host ''Carl'') = {\<lparr>entity = Host ''Alice'', port = Port 1\<rparr>}" by eval
+
+    text{*Dan is not connected*}
+    lemma "send_to_code example_network2 \<lparr>entity = Host ''Alice'', port = Port 1\<rparr> (Host ''Dan'') = {}" by eval
+    
+    text{*the rest and only the rest is reachble without packets beeing send seomwhere undesired*}
+    lemma "\<forall> dst \<in> hosts (interfaces example_network2) - {\<lparr>entity = Host ''Dan'', port = Port 1\<rparr>}.
+        send_to_code example_network2 \<lparr>entity = Host ''Alice'', port = Port 1\<rparr> (entity dst) = {dst}" by eval
 
 
 section{*cleanup namespace*}
